%!TEX program = xelatex
\documentclass[a4papers]{ctexart}
%数学符号
\usepackage{amssymb}
\usepackage{amsmath}
%表格
\usepackage{graphicx,floatrow}
\usepackage{array}
\usepackage{booktabs}
\usepackage{makecell}
%页边距
\usepackage{geometry}
\geometry{left=2cm,right=2cm,top=2cm,bottom=2cm}

%首行缩进两字符 利用\indent \noindent进行控制
\usepackage{indentfirst}
\setlength{\parindent}{2em}

\setromanfont{Songti SC}
%\setromanfont{Heiti SC}

\title{STATS100B--Introduction Mathmatical Statistics \\Homework 1}
\author{Feng Shiwei \ UID:305256428}
\date{}
\begin{document}
\maketitle
\section*{Exercise 1}
\noindent Solution：
\begin{alignat*}{2}
    P(X=x)&=\binom{n}{x}\theta^x(1-\theta)^{n-x}\\
          &=\binom{n}{x}(1-p)^n exp\{{ln\dfrac{p}{1-p}x}\}
\end{alignat*}
so we get
\[c(\boldsymbol{\theta})=(1-p)^n,\, 
\sum_{i=1}^{k}w_i(\boldsymbol{\theta})t_i(x)=ln\dfrac{p}{1-p}x \]
\[
    \sum_{i=1}^{k} \dfrac{\partial w_i(\boldsymbol{\theta})}{\partial \theta_j } t_i(x)    = \dfrac{1}{p(1-p)}x,\,
    \sum_{i=1}^{k} \dfrac{\partial^2 w_i(\boldsymbol{\theta})}{\partial \theta_j^2 } t_i(x)= \dfrac{2p-1}{p^2(1-p)^2}x \]
\[
    \dfrac{\partial^2}{\partial \theta_j^2} logc(\boldsymbol{\theta})=-\dfrac{n}{(1-p)^2} \]
Use the second theorem, we can get the $var(X)$.
\[var( \dfrac{1}{p(1-p) }X) = \dfrac{n}{(1-p)^2} - E(\dfrac{2p-1}{p^2(1-p)^2}X)\]
\[ \dfrac{1}{p^2(1-p)^2}var(X) = \dfrac{n}{(1-p)^2} - \dfrac{2p-1}{p^2(1-p)^2}E(X)
    = \dfrac{n}{(1-p)^2} - \dfrac{2p-1}{p^2(1-p)^2}np \]
\[\therefore var(X)=np(1-p)\]

\section*{Exercise 2}
\noindent Solution:
\[ \int_{x}h(x)c(\boldsymbol{\theta})exp \big\{ \sum_{i=1}^{k}w_i(\boldsymbol{\theta})t_i(x) \big\}dx =1 \]
Differentiate both side w.r.t $\theta_j$, 
\[ \int_{x}\Big[h(x)\dfrac{\partial c(\boldsymbol{\theta})}{\partial \theta_j}exp\big(\sum_{i=1}^{k}w_i(\boldsymbol{\theta})t_i(x)\big)  
    + h(x)c(\boldsymbol{\theta})\sum_{i=1}^{k} \dfrac{\partial w_i(\boldsymbol{\theta})}{\partial \theta_j }t_i(x)exp\big(\sum_{i=1}^{k}w_i(\boldsymbol{\theta})t_i(x)\big)\Big ]dx = 0 \]
\[  
   \int_{x}\sum_{i=1}^{k} \dfrac{\partial w_i(\boldsymbol{\theta})}{\partial \theta_j }t_i(x)\Big[h(x)c(\boldsymbol{\theta})exp\big(\sum_{i=1}^{k}w_i(\boldsymbol{\theta})t_i(x)\big)\Big ]dx
  =- \dfrac{1}{c(\boldsymbol{\theta})} \dfrac{\partial c(\boldsymbol{\theta})}{\partial \theta_j} \int_{x}\Big[h(x)c(\boldsymbol{\theta}) exp\big(\sum_{i=1}^{k}w_i(\boldsymbol{\theta})t_i(x)\big) \Big ]dx
\]
\[
     \int_{x}\sum_{i=1}^{k} \dfrac{\partial w_i(\boldsymbol{\theta})}{\partial \theta_j }t_i(x)f(x)dx
  =- \dfrac{\partial logc(\boldsymbol{\theta})}{\partial \theta_j} \int_{x}f(x)dx
\]
\[
    \because \int_{x}f(x)dx=1
\]
\[
    \therefore E\Bigg( \sum_{i=1}^{k} \dfrac{\partial w_i(\boldsymbol{\theta})}{\partial \theta_j }t_i(x) \Bigg)
  =- \dfrac{\partial logc(\boldsymbol{\theta})}{\partial \theta_j} 
\]
\end{document}